## Exercise 2-32
### Question

For each of the following expressions $f(n)$ find a simple $g(n)$ such that
$f(n) = Î˜(g(n))$.

$$
\begin{align*}
    \text{(a)}\quad&f(n)=\sum_{i=1}^n\frac{1}{i}\\
    \text{(b)}\quad&f(n)=\sum_{i=1}^n\left\lceil\frac{1}{i}\right\rceil\\
    \text{(c)}\quad&f(n)=\sum_{i=1}^n\log{i}\\
    \text{(d)}\quad&f(n)=\log{n!}
\end{align*}
$$


### Solution

### Solution for (a)

As a graph below shows, the summation can be regarded as an uppersum of a function $y=\frac{1}{x}$ and bound by two reciprocal functions.

![two function bindings](https://raw.githubusercontent.com/dede-20191130/tadm-solutions/main/Ch_2_Algorithm_Analysis/tadm_e2-32.png)

And the next inequation holds:


$$
\begin{equation}
    \int_1^n\frac{1}{x}dx \le \sum_{i=1}^n\frac{1}{i} \le \int_2^{n+1}\frac{1}{x-1}dx+1
\end{equation}
$$

Think of solving Left Hand Side and Right hand Side of the above formula.


$$
\begin{align}
    \int_1^n\frac{1}{x}dx &= \left[\ln{|x|}\right]_1^n\\
    &=\ln{n}
\end{align}
$$

$$
\begin{align}
    \int_2^{n+1}\frac{1}{x-1}dx+1 &= \left[\ln{|x-1|}\right]_2^{n+1}+1\\
    &=\ln{n}+1
\end{align}
$$

So, $f(n)$'s boundation and function $g(n)$ is:


$$
\begin{equation}
    f(n)=\Theta(\log{n})
\end{equation}
$$

$$
\begin{equation}
    g(n)=\log{n}
\end{equation}
$$

### Solution for (b)

$$
\begin{equation}
    o \lt \frac{1}{i} \lt 1 \quad \text{for} \{i\in\mathbb{N}\} 
\end{equation}
$$

So, 

$$
\begin{align}
    \left\lceil \frac{1}{i} \right\rceil&=1\\
    f(n)&=\sum_{i=1}^n\left\lceil\frac{1}{i}\right\rceil=n
\end{align}
$$

So function $g(n)$ is:

$$
\begin{equation}
    g(n)=n
\end{equation}
$$


### Solution for (c)

From similar analysis as promlem(a), 

$$
\begin{equation}
    \int_1^n\log{x}dx \lt \sum_{i=1}^n\log{i} \lt \int_2^{n+1}\log{(x-1)}dx+1
\end{equation}
$$

Think of LHS and RHS.  
For simplicity, we think abount $\ln{x}$ rather than $\log{x}$(the asymptotical order is same).

$$
\begin{align}
    LHS&=\int_1^n\ln{x}dx\\
    &=\left[x\ln{x}\right]_1^n-\int_1^n1dx\\
    &=n\ln{n}+\Theta(n)\\
    &=\Theta(n\log{n})
\end{align}
$$

$$
\begin{align}
    RHS&=\int_2^{n+1}\ln{(x-1)}dx+1\\
    &=\left[x\ln{(x-1)}\right]_2^{n+1}-\int_2^{n+1}(1-\frac{1}{n-1})dx+1\\
    &=\Theta(n\ln{n})+\Theta(n)+\Theta(\ln{n})+\Theta(1)\\
    &=\Theta(n\log{n})
\end{align}
$$

So, 

$$
\begin{equation}
    g(n)=n\log{n}
\end{equation}
$$


### Solution for (d)

The product as an anti-logarithm can be distributed into the summation of logarithm.

$$
\begin{align}
    f(n)&=\log{n!}\\
    &=\sum_{i=1}^n\log{i}
\end{align}
$$

The shape of the formula is exactly the same as that in the problem (c).  
So the result is also the same.
