## Exercise 2-21
### Question

Prove that for all k ≥ 0 and all sets of real constants $\{a_k, a_k−1,...,a_1, a_0\}$,  

$a_kn^k + a_{k−1}n^k−1 + .... + a_1n + a_0 = O(n^k)$


### Solution

There are two distinct approaches for this problem.

#### The solution using formula of the sum of geometric seris

<1> The case $n=1$:

$$
\begin{align}
LHS&=Constant.\\
RHS&=O(1)
\end{align}
$$

So the statement holds.

<2> The case $n\ge2$:

$$
\begin{equation}
LHS=a_kn^k+\sum_{i=0}^{k-1}a_in^i
\end{equation}
$$

Set $b$ as:

$$
\begin{equation}
b=\max \{ a_i : i \in \mathbb{Z} \land 0 \leq i \leq k-1 \}
\end{equation}
$$

Amount b derives a new binding below:

$$
\begin{equation}
\sum_{i=0}^{k-1}a_in^i\le b\sum_{i=0}^{k-1}n^i
\end{equation}
$$

We can apply the formula of the sum of geometric seris to this.

$$
\begin{equation}
b\sum_{i=0}^{k-1}n^i=\frac{b(n^k-1)}{n-1}
\end{equation}
$$

Since $n\ge2$,

$$
\begin{equation}
\frac{b(n^k-1)}{n-1}\le b(n^k-1)
\end{equation}
$$

So,

$$
\begin{equation}
b\sum_{i=0}^{k-1}n^i=O(n^k)
\end{equation}
$$

Equation (3), (5) and (8) derive:

$$
\begin{equation}
a_kn^k + a_{k−1}n^k−1 + .... + a_1n + a_0 = O(n^k)
\end{equation}
$$

Using <1> and <2>, the statement holds.


#### The solution using induction

Set $func(m)$ as:

$$
\begin{equation}
func(m)=\sum_{i=0}^{m}a_{k-i}n^{k-i}\qquad\{ 0 \leq m \leq k \}
\end{equation}
$$

We'll prove $func(m)=O(n^k)$ for all $m$.

<1> the case $m=0$

$$
\begin{equation}
func(0)=a_kn^k=O(k)
\end{equation}
$$

<2> induction for $m'$ and $m'+1$

Assume $func(m')=O(n^k)$ when $m=m'$.

Think of $func(m'+1)$.

$$
\begin{equation}
func(m'+1)=func(m')+a_{k-m'-1}n^{k-m'-1}
\end{equation}
$$

The definition of $O$ derives:

$$
\begin{equation}
func(m')\le c_1n^k \:\: \text{for}\:\: n\ge n_1
\end{equation}
$$

And since $n$ is large enough number,

$$
\begin{equation}
n^{k-m'-1}\le n^k
\end{equation}
$$

Statement (12)-(14) derives:

$$
\begin{equation}
func(m'+1)\le (c_1+a_{k-m'-1})n^k \:\: \text{for}\:\: n\ge n_1
\end{equation}
$$

So,

$$
\begin{equation}
func(m'+1)=O(n^k)
\end{equation}
$$

From <1> and <2>, $func(m)=O(n^k)$ is proved.

The pattern

$$
\begin{align}
func(k)&=a_kn^k + a_{k−1}n^k−1 + .... + a_1n + a_0\\
&=O(n^k)
\end{align}
$$

is what we want to prove.