## Exercise 2-22
### Question

Show that for any real constants $a$ and $b$, $b > 0$  

$$
\begin{equation}
(n+a)^b=ʘ(n^b)
\end{equation}
$$


### Solution

There are at least two distinct approaches for this problem.



#### The solution by normal inequation relations

For large enough $n$, $n$ satisfies the following inequation:

$$
\begin{equation}
    n \ge max\{-2a, 2a\}
\end{equation}
$$

\[1\] In that time, $n$ and $a$ satisfies a inequation and both hands of the statement is greater than or equal to 0.

$$
\begin{equation}
    \frac{n}{2} \le n+a
\end{equation}
$$

Raise to the both sides:


$$
\begin{equation}
    \left(\frac{n}{2}\right)^b \le (n+a)^b
\end{equation}
$$

So,

$$
\begin{equation}
    (n+a)^b=\Omega(n^b)
\end{equation}
$$

\[2\] For large enough n, $n \ge a$, so,


$$
\begin{equation}
    (n+a)^b \le (n+n)^b=2^bn^b
\end{equation}
$$

So,

$$
\begin{equation}
    (n+a)^b=O(n^b)
\end{equation}
$$

\[1\] and \[2\] derives:

$$
\begin{equation}
(n+a)^b=ʘ(n^b)
\end{equation}
$$

#### The solution using the result of the previous exercise 2-21

Using binomial expansion to $(n+a)^b$, we get the following statement:

$$
\begin{equation}
(n+a)^b=n^b+\sum_{i=0}^{b-1}a_in^i
\end{equation}
$$

The result of exercise 2-21 says the second term of the left-hand side in above equation is $O(n^{b-1})$.  
So,

$$
\begin{align}
(n+a)^b&=n^b+\sum_{i=0}^{b-1}a_in^i\\
&=\Theta(n^b)+O(n^{b-1})=\Theta(n^b)\:\text{(the answer)}
\end{align}
$$




